src/study/Nemonuri.Study.CSharpSyntaxRewriter2.Modifier/Nemonuri.StratifiedNode.ListTheory.Properties.fst
@@ -65,7 +65,7 @@ let lemma_element_level_is_less_or_equal_than_list_max_level
 let lemma_two_list_are_equal_means_two_heads_are_equal
   (#t:eqtype) (#l_mlv:nat) (l_snl:stratified_node_list t l_mlv{SCons? l_snl})
   (#r_mlv:nat) (r_snl:stratified_node_list t r_mlv{SCons? r_snl})
-  : Lemma (requires is_equal l_snl r_snl)
+  : Lemma (requires is_equal_list l_snl r_snl)
           (ensures (get_hd l_snl) = (get_hd r_snl))
   = ()
 
@@ -76,7 +76,7 @@ let rec lemma_snl1_ends_with_snl2_means_snl1_contains_snl2_head
                     (ends_with snl1 snl2) )
           (ensures contains snl1 (get_hd snl2))
           (decreases snl1)
-  = if (is_equal snl1 snl2) then
+  = if (is_equal_list snl1 snl2) then
       (
         lemma_two_list_are_equal_means_two_heads_are_equal snl1 snl2
       )
@@ -86,7 +86,7 @@ let rec lemma_snl1_ends_with_snl2_means_snl1_contains_snl2_head
 let lemma_two_list_are_equal_means_two_tails_are_equal
   (#t:eqtype) (#l_mlv:nat) (l_snl:stratified_node_list t l_mlv{SCons? l_snl})
   (#r_mlv:nat) (r_snl:stratified_node_list t r_mlv{SCons? r_snl})
-  : Lemma (requires is_equal l_snl r_snl)
+  : Lemma (requires is_equal_list l_snl r_snl)
           (ensures (get_tl l_snl) = (get_tl r_snl))
   = ()
 
@@ -97,7 +97,7 @@ let rec lemma_snl1_ends_with_snl2_means_snl1_ends_with_snl2_tl
                     (ends_with snl1 snl2) )
           (ensures ends_with snl1 (get_tl snl2))
           (decreases snl1)
-  = if (is_equal snl1 snl2) then
+  = if (is_equal_list snl1 snl2) then
       (
         lemma_two_list_are_equal_means_two_tails_are_equal snl1 snl2
       )
